GroupApproximation.lean
@@ -97,6 +97,7 @@ import GroupApproximation.Computability.AmalgamCodePushout
 import GroupApproximation.Computability.BenignMapEmbCode
 import GroupApproximation.Computability.BenignInfCode
 import GroupApproximation.Computability.BenignSupCode
+import GroupApproximation.Computability.BenignComapCode
 import GroupApproximation.Computability.BenignMapEmbRopeInput
 import GroupApproximation.Computability.DirectProductCodeSemantics
 import GroupApproximation.Computability.AdianRabinVariantTransform
